src/Parsers/ExtrOcamlParsers.v
@@ -1,5 +1,5 @@
-Require Import Coq.Arith.Compare_dec.
-Require Import ADTSynthesis.Common.Equality.
+Require Import Coq.Arith.Compare_dec Coq.Strings.String.
+Require Import ADTSynthesis.Common.Equality ADTSynthesis.Parsers.ParserFromParserADT ADTSynthesis.Parsers.SplitterFromParserADT ADTSynthesis.Parsers.ParserInterface.
 Require Export ExtrOcamlBasic.
 Require Export ExtrOcamlNatInt.
 Require Export ExtrOcamlString.
@@ -7,3 +7,25 @@ Extract Inlined Constant Compare_dec.lt_dec => "(<)".
 Extract Inlined Constant Sumbool.sumbool_of_bool => "(fun x -> x)".
 Extract Inlined Constant Equality.ascii_beq => "(=)".
 Extract Inlined Constant ascii_eq_dec => "(=)".
+
+Global Arguments string_dec : simpl never.
+Global Arguments Equality.string_beq : simpl never.
+Global Arguments SplitterFromParserADT.msplits / .
+Global Arguments splits_for / .
+Global Arguments Equality.ascii_beq !_ !_ / .
+Global Arguments SplitterFromParserADT.mlength / .
+Global Arguments SplitterFromParserADT.mis_char / .
+Global Arguments SplitterFromParserADT.mtake / .
+Global Arguments SplitterFromParserADT.mdrop / .
+Global Arguments SplitterFromParserADT.mto_string / .
+Global Arguments new_string_of_string / .
+Global Arguments ComputationalADT.cRep / .
+Global Arguments new_string_of_base_string / .
+Global Arguments ComputationalADT.cConstructors / .
+
+Module HideProofs.
+  Notation hex := (ex _).
+  Notation exist' x := (exist _ x _).
+  Notation horr := (or_intror _).
+  Notation horl := (or_introl _).
+End HideProofs.
