src/Parsers/Refinement/SharpenedABStar.v
@@ -31,51 +31,11 @@ Section IndexedImpl.
 
 End IndexedImpl.
 
+Global Arguments ComputationalSplitter / .
+
 Require Import ADTSynthesis.Parsers.ParserFromParserADT.
 Require Import ADTSynthesis.Parsers.ExtrOcamlParsers.
-
-Local Ltac do_compute_in term hyp :=
-  let term' := (eval compute in term) in
-  change term with term' in hyp.
-
-Local Ltac do_lazy_in term hyp :=
-  let term' := (eval lazy in term) in
-  change term with term' in hyp.
-
-Local Ltac do_simpl_in term hyp :=
-  let term' := (eval simpl in term) in
-  change term with term' in hyp.
-
-Local Ltac do_hnf_in term hyp :=
-  let term' := (eval hnf in term) in
-  change term with term' in hyp.
-
-Local Ltac set_subst_hnf_in term hyp :=
-  let H := fresh in
-  set (H := term) in hyp;
-    hnf in H;
-    cbv beta iota zeta delta [H] in hyp;
-    subst H.
-
-Local Arguments string_dec : simpl never.
-Local Arguments Equality.string_beq : simpl never.
-Arguments SplitterFromParserADT.msplits / .
-Arguments splits_for / .
-Arguments Equality.ascii_beq !_ !_ / .
-Arguments SplitterFromParserADT.mlength / .
-Arguments SplitterFromParserADT.mis_char / .
-Arguments SplitterFromParserADT.mtake / .
-Arguments SplitterFromParserADT.mdrop / .
-Arguments SplitterFromParserADT.mto_string / .
-Arguments new_string_of_string / .
-Arguments ComputationalSplitter / .
-Arguments ComputationalADT.cRep / .
-Arguments new_string_of_base_string / .
-Arguments ComputationalADT.cConstructors / .
-Local Notation hextr0 := (ex _).
-Local Notation exist' x := (exist _ x _).
-Local Notation hextr1 := (or_intror _).
-Local Notation hextr2 := (or_introl _).
+Import ADTSynthesis.Parsers.ExtrOcamlParsers.HideProofs.
 
 Time Definition ab_star_parser (str : String.string) : bool
   := Eval simpl in has_parse (parser ComputationalSplitter) str.
